cfrontend/Cstrategy.v
@@ -142,7 +142,9 @@ Inductive eval_simple_list: exprlist -> typelist -> list val -> Prop :=
   | esrl_nil:
       eval_simple_list Enil Tnil nil
   | esrl_cons: forall r rl ty tyl v vl v',
-      eval_simple_rvalue r v' -> sem_cast v' (typeof r) ty m = Some v ->
+      eval_simple_rvalue r v' -> 
+      is_ptrtoint_cast (typeof r) ty = false ->
+      sem_cast v' (typeof r) ty m = Some v ->
       eval_simple_list rl tyl vl ->
       eval_simple_list (Econs r rl) (Tcons ty tyl) (v :: vl).
 
@@ -291,30 +293,34 @@ Inductive estep: state -> trace -> state -> Prop :=
       estep (ExprState f (C (Econdition r1 r2 r3 ty)) k e m)
          E0 (ExprState f (C (Eparen (if b then r2 else r3) ty ty)) k e m)
 
-  | step_assign: forall f C l r ty k e m b ofs v v' t m',
+  | step_assign: forall f C l r ty k e m b ofs v v' b' ofs' t m' m'',
       leftcontext RV RV C ->
       eval_simple_lvalue e m l b ofs ->
       eval_simple_rvalue e m r v ->
-      sem_cast v (typeof r) (typeof l) m = Some v' ->
-      assign_loc ge (typeof l) m b ofs v' t m' ->
+      (is_ptrtoint_cast (typeof r) (typeof l) = false /\ m' = m) \/
+      (is_ptrtoint_cast (typeof r) (typeof l) = true /\ v = Vptr b' ofs' /\ realize_block m b' m') ->
+      sem_cast v (typeof r) (typeof l) m' = Some v' ->
+      assign_loc ge (typeof l) m' b ofs v' t m'' ->
       ty = typeof l ->
       estep (ExprState f (C (Eassign l r ty)) k e m)
-          t (ExprState f (C (Eval v' ty)) k e m')
+          t (ExprState f (C (Eval v' ty)) k e m'')
 
-  | step_assignop: forall f C op l r tyres ty k e m b ofs v1 v2 v3 v4 t1 t2 m' t,
+  | step_assignop: forall f C op l r tyres ty k e m b ofs b' ofs' v1 v2 v3 v4 t1 t2 m' t m'',
       leftcontext RV RV C ->
       eval_simple_lvalue e m l b ofs ->
       deref_loc ge (typeof l) m b ofs t1 v1 ->
       eval_simple_rvalue e m r v2 ->
       sem_binary_operation ge op v1 (typeof l) v2 (typeof r) m = Some v3 ->
-      sem_cast v3 tyres (typeof l) m = Some v4 ->
-      assign_loc ge (typeof l) m b ofs v4 t2 m' ->
+      (is_ptrtoint_cast tyres (typeof l) = false /\ m' = m) \/
+      (is_ptrtoint_cast tyres (typeof l) = true /\ v3 = Vptr b' ofs' /\ realize_block m b' m') ->
+      sem_cast v3 tyres (typeof l) m' = Some v4 ->
+      assign_loc ge (typeof l) m' b ofs v4 t2 m'' ->
       ty = typeof l ->
       t = t1 ** t2 ->
       estep (ExprState f (C (Eassignop op l r tyres ty)) k e m)
-          t (ExprState f (C (Eval v4 ty)) k e m')
+          t (ExprState f (C (Eval v4 ty)) k e m'')
 
-  | step_assignop_stuck: forall f C op l r tyres ty k e m b ofs v1 v2 t,
+  | step_assignop_stuck: forall f C op l r tyres ty k e m b ofs v1 v2 t m' b' ofs',
       leftcontext RV RV C ->
       eval_simple_lvalue e m l b ofs ->
       deref_loc ge (typeof l) m b ofs t v1 ->
@@ -322,9 +328,11 @@ Inductive estep: state -> trace -> state -> Prop :=
       match sem_binary_operation ge op v1 (typeof l) v2 (typeof r) m with
       | None => True
       | Some v3 =>
-          match sem_cast v3 tyres (typeof l) m with
+          ((is_ptrtoint_cast tyres (typeof l) = false /\ m' = m) \/
+          (is_ptrtoint_cast tyres (typeof l) = true /\ v3 = Vptr b' ofs' /\ realize_block m b' m')) /\
+          match sem_cast v3 tyres (typeof l) m' with
           | None => True
-          | Some v4 => forall t2 m', ~(assign_loc ge (typeof l) m b ofs v4 t2 m')
+          | Some v4 => forall t2 m'', ~(assign_loc ge (typeof l) m b ofs v4 t2 m'')
           end
       end ->
       ty = typeof l ->
@@ -564,8 +572,14 @@ Definition invert_expr_prop (a: expr) (m: mem) : Prop :=
   | Econdition (Eval v1 ty1) r1 r2 ty =>
       exists b, bool_val v1 ty1 m = Some b
   | Eassign (Eloc b ofs ty1) (Eval v2 ty2) ty =>
-      exists v, exists m', exists t,
-      ty = ty1 /\ sem_cast v2 ty2 ty1 m = Some v /\ assign_loc ge ty1 m b ofs v t m'
+      exists v,
+      match is_ptrtoint_cast ty2 ty1 with
+      | true => exists m' t m'' b' ofs',
+        v2 = Vptr b' ofs' /\ realize_block m b' m' /\ ty = ty1 /\
+        sem_cast v2 ty2 ty1 m' = Some v /\ assign_loc ge ty1 m' b ofs v t m''
+      | false => exists m', exists t,
+        ty = ty1 /\ sem_cast v2 ty2 ty1 m = Some v /\ assign_loc ge ty1 m b ofs v t m'
+      end
   | Eassignop op (Eloc b ofs ty1) (Eval v2 ty2) tyres ty =>
       exists t, exists v1,
       ty = ty1
@@ -580,16 +594,16 @@ Definition invert_expr_prop (a: expr) (m: mem) : Prop :=
       exists v, sem_cast v1 ty1 ty2 m = Some v
   | Ecall (Eval vf tyf) rargs ty =>
       exprlist_all_values rargs ->
-      exists tyargs tyres cconv fd vl,
+      exists tyargs tyres cconv fd vl m',
          classify_fun tyf = fun_case_f tyargs tyres cconv
       /\ Genv.find_funct ge vf = Some fd
-      /\ cast_arguments m rargs tyargs vl
+      /\ cast_arguments m' rargs tyargs vl m
       /\ type_of_fundef fd = Tfunction tyargs tyres cconv
   | Ebuiltin ef tyargs rargs ty =>
       exprlist_all_values rargs ->
-      exists vargs, exists t, exists vres, exists m',
-         cast_arguments m rargs tyargs vargs
-      /\ external_call ef ge vargs m t vres m'
+      exists vargs, exists t, exists vres, exists m', exists m'',
+         cast_arguments m rargs tyargs vargs m'
+      /\ external_call ef ge vargs m' t vres m''
   | _ => True
   end.
 
@@ -616,11 +630,16 @@ Proof.
   exists true; auto. exists false; auto.
   exists true; auto. exists false; auto.
   exists b; auto.
-  exists v; exists m'; exists t; auto.
+  exists v. destruct (is_ptrtoint_cast ty2 ty1).
+    destruct H. 
+      destruct H. inversion H. 
+      destruct H. destruct H2. exists m'. exists t. exists m''. exists b'. exists ofs'. tauto.
+      exists m''. exists t. destruct H. destruct H. rewrite H2 in *. tauto.
+      destruct H. inversion H.
   exists t; exists v1; auto.
   exists t; exists v1; auto.
   exists v; auto.
-  intros. exists vargs; exists t; exists vres; exists m'; auto.
+  intros. exists vargs; exists t; exists vres; exists m'; exists m''; auto.
 Qed.
 
 Lemma callred_invert:
@@ -629,7 +648,7 @@ Lemma callred_invert:
   invert_expr_prop r m.
 Proof.
   intros. inv H. simpl.
-  intros. exists tyargs, tyres, cconv, fd, args; auto.
+  intros. exists tyargs, tyres, cconv, fd, args, m0; auto.
 Qed.
 
 Scheme context_ind2 := Minimality for context Sort Prop
@@ -913,25 +932,28 @@ Inductive eval_simple_list': exprlist -> list val -> Prop :=
 Lemma eval_simple_list_implies:
   forall rl tyl vl,
   eval_simple_list e m rl tyl vl ->
-  exists vl', cast_arguments m (rval_list vl' rl) tyl vl /\ eval_simple_list' rl vl'.
+  exists vl', cast_arguments m (rval_list vl' rl) tyl vl m /\ eval_simple_list' rl vl'.
 Proof.
   induction 1.
   exists (@nil val); split. constructor. constructor.
   destruct IHeval_simple_list as [vl' [A B]].
-  exists (v' :: vl'); split. constructor; auto. constructor; auto.
+  exists (v' :: vl'); split.
+  apply cast_args_cons with m 1%positive Ptrofs.zero; eauto.  
+  constructor. auto. auto.
 Qed.
 
+(* JYLEE : This is wrong after addition of realize to cast_arguments. *)
 Lemma can_eval_simple_list:
   forall rl vl,
   eval_simple_list' rl vl ->
   forall tyl vl',
-  cast_arguments m (rval_list vl rl) tyl vl' ->
+  cast_arguments m (rval_list vl rl) tyl vl' m ->
   eval_simple_list e m rl tyl vl'.
 Proof.
   induction 1; simpl; intros.
   inv H. constructor.
-  inv H1. econstructor; eauto.
-Qed.
+  (* inv H1. econstructor ; eauto. *)
+Admitted.
 
 Fixpoint exprlist_app (rl1 rl2: exprlist) : exprlist :=
   match rl1 with
@@ -1210,8 +1232,9 @@ Proof.
   eapply eval_simple_lvalue_steps with (C := fun x => C(Eassign x r (typeof l))); eauto.
   eapply plus_right.
   eapply eval_simple_rvalue_steps with (C := fun x => C(Eassign (Eloc b ofs (typeof l)) x (typeof l))); eauto.
-  left; apply step_rred; eauto. econstructor; eauto.
-  reflexivity. auto.
+  left; apply step_rred; eauto.
+    econstructor. 
+    eapply H3. auto. eauto. eauto. eauto.
 (* assignop *)
   eapply star_plus_trans.
   eapply eval_simple_lvalue_steps with (C := fun x => C(Eassignop op x r tyres (typeof l))); eauto.
@@ -1225,7 +1248,8 @@ Proof.
   left; apply step_rred; auto. econstructor; eauto.
   reflexivity. reflexivity. reflexivity. traceEq.
 (* assignop stuck *)
-  eapply star_plus_trans.
+  admit.
+(*eapply star_plus_trans.
   eapply eval_simple_lvalue_steps with (C := fun x => C(Eassignop op x r tyres (typeof l))); eauto.
   eapply star_plus_trans.
   eapply eval_simple_rvalue_steps with (C := fun x => C(Eassignop op (Eloc b ofs (typeof l)) x tyres (typeof l))); eauto.
@@ -1236,14 +1260,18 @@ Proof.
   left; apply step_rred with (C := fun x => C(Eassign (Eloc b ofs (typeof l)) x (typeof l))); eauto. econstructor; eauto.
   apply star_one.
   left; eapply step_stuck; eauto.
-  red; intros. exploit imm_safe_inv; eauto. simpl. intros [v4' [m' [t' [A [B D]]]]].
+  red; intros. exploit imm_safe_inv; eauto. simpl.
+    destruct (is_ptrtoint_cast tyres (typeof l)) eqn:?.
+    destruct H4. destruct H4. destruct H4. inversion H4.
+      destruct H4. destruct H6.
+      intros [v4' [m''' [t' [m'' [b'' [ofs'' [P [Q [A [B D]]]]]]]]]].
   rewrite B in H4. eelim H4; eauto.
   reflexivity.
   apply star_one.
   left; eapply step_stuck with (C := fun x => C(Eassign (Eloc b ofs (typeof l)) x (typeof l))); eauto.
   red; intros. exploit imm_safe_inv; eauto. simpl. intros [v3 A]. congruence.
   reflexivity.
-  reflexivity. traceEq.
+  reflexivity. traceEq. *)
 (* postincr *)
   eapply star_plus_trans.
   eapply eval_simple_lvalue_steps with (C := fun x => C(Epostincr id x (typeof l))); eauto.
@@ -1255,11 +1283,13 @@ Proof.
   eapply star_left.
   left; apply step_rred with (C := fun x => C (Ecomma x (Eval v1 (typeof l)) (typeof l))); eauto.
   econstructor; eauto.
+  admit.
   apply star_one.
   left; apply step_rred; auto. econstructor; eauto.
   reflexivity. reflexivity. reflexivity. traceEq.
 (* postincr stuck *)
-  eapply star_plus_trans.
+  admit.
+(*eapply star_plus_trans.
   eapply eval_simple_lvalue_steps with (C := fun x => C(Epostincr id x (typeof l))); eauto.
   eapply plus_left.
   left; apply step_rred; auto. econstructor; eauto.
@@ -1280,7 +1310,7 @@ Proof.
   left; eapply step_stuck with (C := fun x => C (Ecomma (Eassign (Eloc b ofs (typeof l)) x (typeof l)) (Eval v1 (typeof l)) (typeof l))); eauto.
   red; intros. exploit imm_safe_inv; eauto. simpl. intros [v2 A]. congruence.
   reflexivity.
-  traceEq.
+  traceEq.*)
 (* comma *)
   eapply plus_right.
   eapply eval_simple_rvalue_steps with (C := fun x => C(Ecomma x r2 (typeof r2))); eauto.
@@ -1305,14 +1335,15 @@ Proof.
   eapply contextlist'_builtin with (rl0 := Enil); auto.
   left; apply Csem.step_rred; eauto. econstructor; eauto.
   traceEq.
-Qed.
+Admitted.
 
 Lemma can_estep:
   forall f a k e m,
   safe (ExprState f a k e m) ->
   match a with Eval _ _ => False | _ => True end ->
   exists t, exists S, estep (ExprState f a k e m) t S.
-Proof.
+Admitted.
+(* Proof.
   intros. destruct (decompose_topexpr f k e m a H) as [A | [C [b [P [Q R]]]]].
 (* simple expr *)
   exploit (simple_can_eval f k e m a RV (fun x => x)); auto. intros [v P].
@@ -1430,7 +1461,7 @@ Proof.
   intros [v1 [E1 S1]].
   exploit safe_inv. eexact S1. eauto. simpl. intros [v CAST].
   econstructor; econstructor; eapply step_paren; eauto.
-Qed.
+Qed.*)
 
 (** Simulation for all states *)
 
@@ -1520,6 +1551,8 @@ Qed.
 
 Lemma semantics_strongly_receptive:
   forall p, strongly_receptive (semantics p).
+Admitted.
+(*
 Proof.
   intros. constructor; simpl; intros.
 (* receptiveness *)
@@ -1627,7 +1660,7 @@ Proof.
   (* external calls *)
   exploit external_call_trace_length; eauto.
   destruct t; simpl; auto. destruct t; simpl; auto. intros; omegaContradiction.
-Qed.
+Qed.*)
 
 (** The main simulation result. *)
 
@@ -2263,6 +2296,8 @@ Lemma bigstep_to_steps:
    forall k,
    is_call_cont k ->
    star step ge (Callstate fd args k m) t (Returnstate res k m')).
+Admitted.
+(*
 Proof.
   apply bigstep_induction; intros.
 (* expression, general *)
@@ -2688,6 +2723,7 @@ Proof.
 (* call external *)
   apply star_one. right; apply step_external_function; auto.
 Qed.
+*)
 
 Lemma eval_expression_to_steps:
    forall e m a t m' v,
